proofmode/pviewshifts.v
@@ -7,6 +7,9 @@ Section pvs.
 Context {Λ : language} {Σ : iFunctor}.
 Implicit Types P Q : iProp Λ Σ.
 
+Global Instance to_assumption_pvs E p P Q :
+  ToAssumption p P Q → ToAssumption p P (|={E}=> Q)%I.
+Proof. rewrite /ToAssumption=>->. apply pvs_intro. Qed.
 Global Instance sep_split_pvs E P Q1 Q2 :
   SepSplit P Q1 Q2 → SepSplit (|={E}=> P) (|={E}=> Q1) (|={E}=> Q2).
 Proof. rewrite /SepSplit=><-. apply pvs_sep. Qed.
